gravy/src/org/gravy/report/InterpolationInfeasibleReport.java
@@ -3,13 +3,17 @@
  */
 package org.gravy.report;
 
+import java.util.HashMap;
+import java.util.LinkedList;
 import java.util.Set;
 
 import org.gravy.faultlocalization.InfeasibleCodeFaultLocalization;
+import org.gravy.util.JavaSourceLocation;
 import org.gravy.verificationcondition.AbstractTransitionRelation;
 
 import boogie.controlflow.AbstractControlFlowFactory;
 import boogie.controlflow.BasicBlock;
+import boogie.controlflow.statement.CfgStatement;
 
 /**
  * @author schaef
@@ -17,10 +21,16 @@ import boogie.controlflow.BasicBlock;
  */
 public class InterpolationInfeasibleReport extends Report {
 
+	private LinkedList<HashMap<CfgStatement, JavaSourceLocation>> reports = new LinkedList<HashMap<CfgStatement, JavaSourceLocation>>();
+	
 	public InterpolationInfeasibleReport(AbstractControlFlowFactory cff,
 			AbstractTransitionRelation tr, Set<BasicBlock> feasibleBlocks,
 			Set<BasicBlock> infeasibleBlocks) {
-		InfeasibleCodeFaultLocalization.localizeFaults(tr, infeasibleBlocks);
+		this.reports = InfeasibleCodeFaultLocalization.localizeFaults(tr, infeasibleBlocks);
 	}	
+	
+	public LinkedList<HashMap<CfgStatement, JavaSourceLocation>> getReports() {
+		return this.reports;
+	}
 	
 }
