gravy/src/org/gravy/reportprinter/InterpolatingInfeasibleCodeReportPrinter.java
@@ -1,0 +1,66 @@
+/**
+ * 
+ */
+package org.gravy.reportprinter;
+
+import java.util.HashMap;
+import java.util.LinkedList;
+import java.util.Map.Entry;
+
+import org.gravy.report.InterpolationInfeasibleReport;
+import org.gravy.report.Report;
+import org.gravy.util.JavaSourceLocation;
+
+import util.Log;
+import boogie.controlflow.statement.CfgStatement;
+
+/**
+ * @author schaef
+ *
+ */
+public class InterpolatingInfeasibleCodeReportPrinter implements ReportPrinter {
+
+	/**
+	 * 
+	 */
+	public InterpolatingInfeasibleCodeReportPrinter() {
+		// TODO Auto-generated constructor stub
+	}
+
+	/* (non-Javadoc)
+	 * @see org.gravy.reportprinter.ReportPrinter#printReport(org.gravy.report.Report)
+	 */
+	@Override
+	public void printReport(Report r) {
+		if (r!=null && r instanceof InterpolationInfeasibleReport) {
+			InterpolationInfeasibleReport ir = (InterpolationInfeasibleReport)r;
+			String s = this.buildBoogieErrorString(ir);
+			if (s!=null && s.length()>0) Log.info(s);
+		}
+	}
+
+	private String buildBoogieErrorString(InterpolationInfeasibleReport ir) {
+		LinkedList<HashMap<CfgStatement, JavaSourceLocation>> reports = ir.getReports();
+		StringBuffer sb = new StringBuffer();
+	
+		sb.append("Total reports: "+reports.size()+ " -----------------\n");
+		int count =0;
+		for (HashMap<CfgStatement, JavaSourceLocation> lines : reports) {
+			sb.append("  Reports: "+(++count));
+			boolean first = true;
+			for (Entry<CfgStatement, JavaSourceLocation> line : lines.entrySet()) {
+				if (first) {
+					sb.append("  In file: " + line.getValue().FileName+"\n");
+					first = false;
+				}
+				sb.append("\t line: " + line.getValue().StartLine+":"+line.getValue().StartCol+"  "+line.getValue().inInfeasibleBlock+"\n");
+				
+			}
+		}
+		
+		return sb.toString();
+	}
+
+
+	
+}
