gravy/test/out.bpl
@@ -96,6 +96,432 @@ procedure void$InfeasibleCode01$$la$init$ra$$1898($this:ref) returns ($exception
 
 procedure void$java.lang.Object$$la$init$ra$$38($this:ref) returns ($exception:ref);    
 
+implementation boolean$InfeasibleCode01$foo$1889($this:ref, $in_parameter__0:ref) returns ($return:int, $exception:ref){
+    
+var temp$710 : int;    
+var temp$69 : int;    
+var this1 : ref;    
+var temp$03 : ref;    
+var temp$14 : ref;    
+var temp$58 : ref;    
+var temp$25 : int;    
+var other2 : ref;    
+var temp$47 : int;    
+var temp$36 : ref;    
+var temp$811 : int;
+    assume { :sourceloc "a.java",-1,-1,-1,-1 } $this != $null;
+    assume $heap[$in_parameter__0,$type] <: InfeasibleCode01;
+    assert { :sourceloc "a.java",10,2,24,2 } true;
+    this1 := $this;
+    assert { :sourceloc "a.java",10,14,10,35 } true;
+    other2 := $in_parameter__0;
+    assert { :sourceloc "a.java",11,7,11,11 } true;
+    temp$03 := $heap[this1,InfeasibleCode01$InfeasibleCode01$bases234];
+    assert { :sourceloc "a.java",11,7,11,11 } true;
+    if (temp$03 == $null) {
+        assert { :sourceloc "a.java",11,7,11,11 } { :comment "thenblock" } true;
+        goto block1;
+    } else {
+        assert { :sourceloc "a.java",12,8,12,26 } { :comment "elseblock" } true;
+    }
+    assert { :sourceloc "a.java",11,7,11,11 } true;
+    goto block2;
+  block1:
+    assert { :sourceloc "a.java",12,8,12,26 } true;
+    assert { :sourceloc "a.java",12,8,12,26 } other2 != $null;
+    temp$14 := $heap[other2,InfeasibleCode01$InfeasibleCode01$bases234];
+    assert { :sourceloc "a.java",12,8,12,26 } true;
+    if (temp$14 != $null) {
+        assert { :sourceloc "a.java",12,8,12,26 } { :comment "thenblock" } true;
+        goto block3;
+    } else {
+        assert { :sourceloc "a.java",12,8,12,26 } { :comment "elseblock" } true;
+    }
+    assert { :sourceloc "a.java",12,8,12,26 } true;
+    goto block2;
+  block3:
+    assert { :sourceloc "a.java",12,8,12,26 } true;
+    temp$25 := 0;
+    assert { :sourceloc "a.java",13,5,13,17 } true;
+    $return := temp$25;
+    return;
+  block2:
+    assert { :sourceloc "a.java",16,7,16,11 } true;
+    temp$36 := $heap[this1,InfeasibleCode01$InfeasibleCode01$bases234];
+    assert { :sourceloc "a.java",16,7,16,11 } true;
+    assert { :sourceloc "a.java",16,7,16,11 } temp$36 != $null;
+    call temp$47, $exception := int$java.lang.Object$hashCode$41(temp$36);
+    assert { :sourceloc "a.java",16,7,16,11 } true;
+    assert { :sourceloc "a.java",16,7,16,11 } other2 != $null;
+    temp$58 := $heap[other2,InfeasibleCode01$InfeasibleCode01$bases234];
+    assert { :sourceloc "a.java",16,7,16,11 } true;
+    assert { :sourceloc "a.java",16,7,16,11 } temp$58 != $null;
+    call temp$69, $exception := int$java.lang.Object$hashCode$41(temp$58);
+    assert { :sourceloc "a.java",16,7,16,11 } true;
+    if (temp$47 != temp$69) {
+        assert { :sourceloc "a.java",16,7,16,11 } { :comment "thenblock" } true;
+        goto block4;
+    } else {
+        assert { :sourceloc "a.java",16,7,16,11 } { :comment "elseblock" } true;
+    }
+    assert { :sourceloc "a.java",16,7,16,11 } true;
+    goto block5;
+  block4:
+    assert { :sourceloc "a.java",16,7,16,11 } true;
+    temp$710 := 0;
+    assert { :sourceloc "a.java",17,4,17,16 } true;
+    $return := temp$710;
+    return;
+  block5:
+    assert { :sourceloc "a.java",17,4,17,16 } true;
+    temp$811 := 1;
+    assert { :sourceloc "a.java",23,3,23,14 } true;
+    $return := temp$811;
+    return;
+}
+
+
+implementation int$InfeasibleCode01$infeasible0$1890($this:ref, $in_parameter__0:ref) returns ($return:int, $exception:ref){
+    
+var temp$318 : ref;    
+var arr13 : ref;    
+var temp$419 : int;    
+var this12 : ref;    
+var temp$116 : int;    
+var i14 : int;    
+var temp$015 : ref;    
+var temp$520 : int;    
+var temp$217 : int;
+    assume { :sourceloc "a.java",-1,-1,-1,-1 } $this != $null;
+    assert { :sourceloc "a.java",27,2,31,2 } true;
+    this12 := $this;
+    assert { :sourceloc "a.java",27,25,27,33 } true;
+    arr13 := $in_parameter__0;
+    assert { :sourceloc "a.java",28,3,28,21 } true;
+    assert { :sourceloc "a.java",28,3,28,21 } arr13 != $null;
+    i14 := $arrSizeHeap[arr13];
+    assert { :sourceloc "a.java",29,3,29,11 } true;
+    temp$015 := arr13;
+    assert { :sourceloc "a.java",29,3,29,11 } true;
+    temp$116 := 3;
+    assert { :sourceloc "a.java",29,6,29,8 } true;
+    temp$217 := 3;
+    assert { :sourceloc "a.java",29,6,29,8 } true;
+    assert { :sourceloc "a.java",29,6,29,8 } temp$116 < $arrSizeHeap[temp$015] && temp$116 >= 0;
+    $intArrHeap := $intArrHeap[temp$015 := $intArrHeap[temp$015][temp$116 := temp$217]];
+    assert { :sourceloc "a.java",29,6,29,8 } true;
+    temp$318 := arr13;
+    assert { :sourceloc "a.java",29,6,29,8 } true;
+    temp$419 := i14;
+    assert { :sourceloc "a.java",29,6,29,8 } true;
+    assert { :sourceloc "a.java",29,6,29,8 } temp$419 < $arrSizeHeap[temp$318] && temp$419 >= 0;
+    temp$520 := $intArrHeap[temp$318][temp$419];
+    assert { :sourceloc "a.java",30,3,30,16 } true;
+    $return := temp$520;
+    return;
+}
+
+
+implementation int$InfeasibleCode01$infeasible1$1891($this:ref, $in_parameter__0:ref) returns ($return:int, $exception:ref){
+    
+var $fakelocal_0 : ref;    
+var temp$528 : int;    
+var $fakelocal_2 : ref;    
+var $fakelocal_1 : ref;    
+var temp$326 : ref;    
+var temp$124 : ref;    
+var this21 : ref;    
+var temp$225 : ref;    
+var temp$427 : ref;    
+var temp$023 : int;    
+var o22 : ref;
+    assume { :sourceloc "a.java",-1,-1,-1,-1 } $this != $null;
+    assume $heap[$in_parameter__0,$type] <: java.lang.Object;
+    assert { :sourceloc "a.java",33,2,39,2 } true;
+    this21 := $this;
+    assert { :sourceloc "a.java",33,25,33,32 } true;
+    o22 := $in_parameter__0;
+    assert { :sourceloc "a.java",34,7,34,13 } true;
+    if (o22 != $null) {
+        assert { :sourceloc "a.java",34,7,34,13 } { :comment "thenblock" } true;
+        goto block6;
+    } else {
+        assert { :sourceloc "a.java",34,7,34,13 } { :comment "elseblock" } true;
+    }
+    assert { :sourceloc "a.java",34,7,34,13 } true;
+    goto block7;
+  block6:
+    assert { :sourceloc "a.java",34,7,34,13 } true;
+    call temp$023, $exception := int$java.lang.Object$hashCode$41(o22);
+    assert { :sourceloc "a.java",35,4,35,23 } true;
+    $return := temp$023;
+    return;
+  block7:
+    assert { :sourceloc "a.java",37,3,37,55 } true;
+    temp$124 := java.io.PrintStream$java.lang.System$err237;
+    assert { :sourceloc "a.java",37,3,37,55 } true;
+    call $fakelocal_0 := $new(java.lang.StringBuffer);
+    temp$225 := $fakelocal_0;
+    assert { :sourceloc "a.java",37,22,37,53 } true;
+    call $exception := void$java.lang.StringBuffer$$la$init$ra$$685(temp$225);
+    assert { :sourceloc "a.java",37,22,37,53 } true;
+    assert { :sourceloc "a.java",37,22,37,53 } o22 != $null;
+    call temp$326, $exception := java.lang.String$java.lang.Object$toString$44(o22);
+    assert { :sourceloc "a.java",37,22,37,53 } true;
+    call $fakelocal_1, $exception := java.lang.StringBuffer$java.lang.StringBuffer$append$701(temp$225, temp$326);
+    assert { :sourceloc "a.java",37,22,37,53 } true;
+    call $fakelocal_2, $exception := java.lang.StringBuffer$java.lang.StringBuffer$append$701(temp$225, $StringConst0);
+    assert { :sourceloc "a.java",37,22,37,53 } true;
+    call temp$427, $exception := java.lang.String$java.lang.StringBuffer$toString$738(temp$225);
+    assert { :sourceloc "a.java",37,22,37,53 } true;
+    assert { :sourceloc "a.java",37,22,37,53 } temp$124 != $null;
+    call $exception := void$java.io.PrintStream$println$217(temp$124, temp$427);
+    assert { :sourceloc "a.java",37,22,37,53 } true;
+    temp$528 := 2;
+    assert { :sourceloc "a.java",38,3,38,11 } true;
+    $return := temp$528;
+    return;
+}
+
+
+implementation void$InfeasibleCode01$infeasible2$1892($this:ref, $in_parameter__0:ref) returns ($exception:ref){
+    
+var temp$436 : int;    
+var temp$335 : int;    
+var temp$133 : ref;    
+var this29 : ref;    
+var temp$032 : int;    
+var arr30 : ref;    
+var i31 : int;    
+var temp$234 : int;
+    assume { :sourceloc "a.java",-1,-1,-1,-1 } $this != $null;
+    assert { :sourceloc "a.java",41,2,45,2 } true;
+    this29 := $this;
+    assert { :sourceloc "a.java",41,26,41,35 } true;
+    arr30 := $in_parameter__0;
+    assert { :sourceloc "a.java",42,8,42,14 } true;
+    i31 := 0;
+  block8:
+    assert { :sourceloc "a.java",42,17,42,29 } true;
+    assert { :sourceloc "a.java",42,17,42,29 } arr30 != $null;
+    temp$032 := $arrSizeHeap[arr30];
+    assert { :sourceloc "a.java",42,17,42,29 } true;
+    if (i31 <= temp$032) {
+        assert { :sourceloc "a.java",42,17,42,29 } { :comment "thenblock" } true;
+        goto block9;
+    } else {
+        assert { :sourceloc "a.java",43,4,43,12 } { :comment "elseblock" } true;
+    }
+    assert { :sourceloc "a.java",42,17,42,29 } true;
+    goto block10;
+  block9:
+    assert { :sourceloc "a.java",43,4,43,12 } true;
+    temp$133 := arr30;
+    assert { :sourceloc "a.java",43,4,43,12 } true;
+    temp$234 := i31;
+    assert { :sourceloc "a.java",43,7,43,9 } true;
+    assert { :sourceloc "a.java",43,7,43,9 } temp$234 < $arrSizeHeap[temp$133] && temp$234 >= 0;
+    $intArrHeap := $intArrHeap[temp$133 := $intArrHeap[temp$133][temp$234 := i31]];
+    assert { :sourceloc "a.java",42,31,42,33 } true;
+    temp$335 := i31;
+    assert { :sourceloc "a.java",42,31,42,31 } true;
+    temp$436 := temp$335 + 1;
+    assert { :sourceloc "a.java",42,31,42,31 } true;
+    i31 := temp$436;
+    assert { :sourceloc "a.java",42,3,44,3 } true;
+    goto block8;
+  block10:
+    assert { :sourceloc "a.java",42,3,44,3 } true;
+    return;
+}
+
+
+implementation void$InfeasibleCode01$infeasible3$1893($this:ref, $in_parameter__0:int, $in_parameter__1:int) returns ($exception:ref){
+    
+var temp$040 : int;    
+var temp$444 : int;    
+var temp$545 : int;    
+var temp$141 : int;    
+var this37 : ref;    
+var temp$343 : int;    
+var b39 : int;    
+var a38 : int;    
+var temp$242 : int;
+    assume { :sourceloc "a.java",-1,-1,-1,-1 } $this != $null;
+    assert { :sourceloc "a.java",47,2,52,2 } true;
+    this37 := $this;
+    assert { :sourceloc "a.java",47,26,47,30 } true;
+    a38 := $in_parameter__0;
+    assert { :sourceloc "a.java",47,33,47,37 } true;
+    b39 := $in_parameter__1;
+    assert { :sourceloc "a.java",48,3,48,3 } true;
+    temp$040 := 1;
+    assert { :sourceloc "a.java",48,3,48,3 } true;
+    b39 := temp$040;
+    assert { :sourceloc "a.java",49,7,49,9 } true;
+    if (a38 > 0) {
+        assert { :sourceloc "a.java",49,7,49,9 } { :comment "thenblock" } true;
+        goto block11;
+    } else {
+        assert { :sourceloc "a.java",49,12,49,15 } { :comment "elseblock" } true;
+    }
+    assert { :sourceloc "a.java",49,7,49,9 } true;
+    goto block12;
+  block11:
+    assert { :sourceloc "a.java",49,12,49,15 } true;
+    temp$141 := b39;
+    assert { :sourceloc "a.java",49,12,49,12 } true;
+    temp$242 := temp$141 + -1;
+    assert { :sourceloc "a.java",49,12,49,12 } true;
+    b39 := temp$242;
+  block12:
+    assert { :sourceloc "a.java",50,3,50,8 } true;
+    assert { :sourceloc "a.java",50,3,50,8 } b39 != 0;
+    temp$343 := 1 div b39;
+    assert { :sourceloc "a.java",50,3,50,3 } true;
+    b39 := temp$343;
+    assert { :sourceloc "a.java",51,7,51,10 } true;
+    if (a38 <= 0) {
+        assert { :sourceloc "a.java",51,7,51,10 } { :comment "thenblock" } true;
+        goto block13;
+    } else {
+        assert { :sourceloc "a.java",51,13,51,22 } { :comment "elseblock" } true;
+    }
+    assert { :sourceloc "a.java",51,7,51,10 } true;
+    goto block14;
+  block13:
+    assert { :sourceloc "a.java",51,13,51,22 } true;
+    temp$444 := 1 - b39;
+    assert { :sourceloc "a.java",51,13,51,22 } true;
+    assert { :sourceloc "a.java",51,13,51,22 } temp$444 != 0;
+    temp$545 := 1 div temp$444;
+  block14:
+    assert { :sourceloc "a.java",51,13,51,13 } true;
+    return;
+}
+
+
+implementation boolean$InfeasibleCode01$infeasible4$1894($this:ref, $in_parameter__0:ref) returns ($return:int, $exception:ref){
+    
+var this46 : ref;    
+var temp$048 : ref;    
+var temp$149 : ref;    
+var o47 : ref;    
+var temp$250 : int;    
+var temp$351 : int;
+    assume { :sourceloc "a.java",-1,-1,-1,-1 } $this != $null;
+    assume $heap[$in_parameter__0,$type] <: java.lang.Object;
+    assert { :sourceloc "a.java",54,2,60,2 } true;
+    this46 := $this;
+    assert { :sourceloc "a.java",54,29,54,36 } true;
+    o47 := $in_parameter__0;
+    assert { :sourceloc "a.java",55,3,55,35 } true;
+    temp$048 := java.io.PrintStream$java.lang.System$err237;
+    assert { :sourceloc "a.java",55,3,55,35 } true;
+    assert { :sourceloc "a.java",55,3,55,35 } o47 != $null;
+    call temp$149, $exception := java.lang.String$java.lang.Object$toString$44(o47);
+    assert { :sourceloc "a.java",55,3,55,35 } true;
+    assert { :sourceloc "a.java",55,3,55,35 } temp$048 != $null;
+    call $exception := void$java.io.PrintStream$println$217(temp$048, temp$149);
+    assert { :sourceloc "a.java",56,7,56,13 } true;
+    if (o47 == $null) {
+        assert { :sourceloc "a.java",56,7,56,13 } { :comment "thenblock" } true;
+        goto block15;
+    } else {
+        assert { :sourceloc "a.java",56,7,56,13 } { :comment "elseblock" } true;
+    }
+    assert { :sourceloc "a.java",56,7,56,13 } true;
+    goto block16;
+  block15:
+    assert { :sourceloc "a.java",56,7,56,13 } true;
+    temp$250 := 0;
+    assert { :sourceloc "a.java",57,4,57,16 } true;
+    $return := temp$250;
+    return;
+  block16:
+    assert { :sourceloc "a.java",57,4,57,16 } true;
+    temp$351 := 1;
+    assert { :sourceloc "a.java",59,3,59,14 } true;
+    $return := temp$351;
+    return;
+}
+
+
+implementation void$InfeasibleCode01$infeasible5$1895($this:ref) returns ($exception:ref){
+    
+var $fakelocal_0 : ref;    
+var this52 : ref;    
+var temp$054 : int;    
+var test53 : ref;    
+var temp$155 : ref;
+    assume { :sourceloc "a.java",-1,-1,-1,-1 } $this != $null;
+    assert { :sourceloc "a.java",62,2,67,2 } true;
+    this52 := $this;
+    assert { :sourceloc "a.java",63,3,63,25 } true;
+    call $fakelocal_0 := $new(java.lang.String);
+    $stringSizeHeap := $stringSizeHeap[$fakelocal_0 := 8];
+    test53 := $fakelocal_0;
+    assert { :sourceloc "a.java",64,7,64,22 } true;
+    temp$054 := $stringSizeHeap[test53];
+    assert { :sourceloc "a.java",64,7,64,22 } true;
+    if (temp$054 == 3) {
+        assert { :sourceloc "a.java",64,7,64,22 } { :comment "thenblock" } true;
+        goto block17;
+    } else {
+        assert { :sourceloc "a.java",65,4,65,37 } { :comment "elseblock" } true;
+    }
+    assert { :sourceloc "a.java",64,7,64,22 } true;
+    goto block18;
+  block17:
+    assert { :sourceloc "a.java",65,4,65,37 } true;
+    temp$155 := java.io.PrintStream$java.lang.System$err237;
+    assert { :sourceloc "a.java",65,4,65,37 } true;
+    assert { :sourceloc "a.java",65,4,65,37 } temp$155 != $null;
+    call $exception := void$java.io.PrintStream$println$217(temp$155, $StringConst1);
+  block18:
+    assert { :sourceloc "a.java",65,4,65,37 } true;
+    return;
+}
+
+
+implementation int$InfeasibleCode01$infeasible6$1896($this:ref, $in_parameter__0:ref) returns ($return:int, $exception:ref){
+    
+var temp$260 : int;    
+var temp$462 : int;    
+var temp$361 : ref;    
+var temp$159 : int;    
+var arr57 : ref;    
+var temp$563 : int;    
+var temp$664 : int;    
+var this56 : ref;    
+var temp$058 : ref;
+    assume { :sourceloc "a.java",-1,-1,-1,-1 } $this != $null;
+    assert { :sourceloc "a.java",69,2,71,2 } true;
+    this56 := $this;
+    assert { :sourceloc "a.java",69,25,69,33 } true;
+    arr57 := $in_parameter__0;
+    assert { :sourceloc "a.java",69,25,69,33 } true;
+    temp$058 := arr57;
+    assert { :sourceloc "a.java",69,25,69,33 } true;
+    temp$159 := -1;
+    assert { :sourceloc "a.java",69,25,69,33 } true;
+    assert { :sourceloc "a.java",69,25,69,33 } temp$159 < $arrSizeHeap[temp$058] && temp$159 >= 0;
+    temp$260 := $intArrHeap[temp$058][temp$159];
+    assert { :sourceloc "a.java",69,25,69,33 } true;
+    temp$361 := arr57;
+    assert { :sourceloc "a.java",69,25,69,33 } true;
+    assert { :sourceloc "a.java",69,25,69,33 } arr57 != $null;
+    temp$462 := $arrSizeHeap[arr57];
+    assert { :sourceloc "a.java",69,25,69,33 } true;
+    assert { :sourceloc "a.java",69,25,69,33 } temp$462 < $arrSizeHeap[temp$361] && temp$462 >= 0;
+    temp$563 := $intArrHeap[temp$361][temp$462];
+    assert { :sourceloc "a.java",69,25,69,33 } true;
+    temp$664 := temp$260 + temp$563;
+    assert { :sourceloc "a.java",70,3,70,35 } true;
+    $return := temp$664;
+    return;
+}
+
 
 implementation void$InfeasibleCode01$infeasible07$1897($this:ref, $in_parameter__0:ref) returns ($exception:ref){
     
@@ -193,4 +619,18 @@ var temp$575 : int;
     assert { :sourceloc "a.java",84,4,84,8 } true;
     return;
 }
+
+
+implementation void$InfeasibleCode01$$la$init$ra$$1898($this:ref) returns ($exception:ref){
+    
+var this80 : ref;
+    assume { :sourceloc "a.java",-1,-1,-1,-1 } $this != $null;
+    assert { :sourceloc "a.java",7,-1,-1,-1 } true;
+    this80 := $this;
+    assert { :sourceloc "a.java",7,-1,-1,-1 } true;
+    call $exception := void$java.lang.Object$$la$init$ra$$38(this80);
+    assert { :sourceloc "a.java",7,-1,-1,-1 } true;
+    return;
+}
+
 
